\section{Energy}
\begin{align}
\langle K \rangle &= -\frac{1}{2}\int \frac{\nabla_{r_1}^2 \psi}{\psi} |\psi|^2 d^3 r_1 d^3 r_2 -\frac{1}{2}\int \frac{\nabla_{r_2}^2 \psi}{\psi} |\psi|^2 d^3 r_1 d^3 r_2 \\
&= -\frac{1}{2} \int_0^{\infty}  \left(-\frac{2 \alpha}{r_1} + \alpha^2\right) \exp(-2 \alpha r_1) 4 r_1^2 dr_1 \int_0^{\infty}\exp(-2 \alpha r_2) 4r_2^2 dr_2 + \cdots \\
&= -\frac{1}{2} \left(-\frac{1}{\alpha}\right) \frac{1}{\alpha^3} -\frac{1}{2} \left(-\frac{1}{\alpha}\right) \frac{1}{\alpha^3} \\
&= \boxed{\frac{1}{\alpha^4}}.
\end{align}

\begin{align}
\langle V_{\mathrm{en}} \rangle &= -Z\int \frac{1}{r_1} \exp(-2 \alpha r_1) \exp(-2 \alpha r_2) d^3 r_1 d^3 r_2 - \cdots \\
&= -Z\int_0^{\infty} \frac{1}{r_1} \exp(-2 \alpha r_1) 4r_1^2 dr_1 \int_0^{\infty} \exp(-2 \alpha r_2) 4 r_2^2 d r_2 - \cdots \\
&= -Z \left(\frac{1}{\alpha^2} \right) \left(\frac{1}{\alpha^3} \right) -Z \left(\frac{1}{\alpha^2} \right) \left(\frac{1}{\alpha^3} \right) \\
&= \boxed{-\frac{2Z}{\alpha^5}}.
\end{align}